oa

VCVio/OracleComp/OracleAlg.lean
@@ -21,27 +21,23 @@ open OracleSpec OracleComp
 
 structure OracleAlg {ι : Type} (spec : ℕ → OracleSpec ι) where
   baseState (n : ℕ) : Type
-  init_state (n : ℕ) : baseState sp
-  baseSimOracle (n : ℕ) : spec n →[baseState sp]ₛₒ unifSpec
-
-structure Protocol {ι : Type} (spec : ℕ → OracleSpec ι) where
-  baseState (n : ℕ) : Type
-  init_state (n : ℕ) : baseState sp
+  init_state (n : ℕ) : baseState n
   baseSimOracle (n : ℕ) : spec n →[baseState n]ₛₒ unifSpec
 
 namespace OracleAlg
 
 variable {ι : Type} {spec : ℕ → OracleSpec ι} {α β γ : Type}
+  (alg : OracleAlg spec) (n : ℕ)
 
 def exec (alg : OracleAlg spec) (n : ℕ)
-    (oa : OracleComp (spec sp) α) : OracleComp unifSpec α :=
-  simulate' (alg.baseSimOracle sp) (alg.init_state sp) oa
+    (oa : OracleComp (spec n) α) : OracleComp unifSpec α :=
+  simulate' (alg.baseSimOracle n) (alg.init_state n) oa
 
--- lemma exec.def (alg : OracleAlg spec) (α : Type) :
---     alg.exec (α := α) = simulate' alg.baseSimOracle alg.init_state := rfl
+lemma exec_def (oa : OracleComp (spec n) α) :
+    alg.exec n oa = simulate' (alg.baseSimOracle n) (alg.init_state n) oa := rfl
 
--- @[simp low]
--- lemma exec_pure (alg : OracleAlg spec) (x : α) : alg.exec (pure x) = pure x := rfl
+@[simp low]
+lemma exec_return (x : α) : alg.exec n (return x) = return x := rfl
 
 -- @[simp low]
 -- lemma exec_bind (alg : OracleAlg spec) (oa : OracleComp spec α) (ob : α → OracleComp spec β) :
@@ -77,10 +73,10 @@ def baseOracleAlg : OracleAlg (λ _ ↦ unifSpec) where
   init_state := λ _ ↦ ()
   baseSimOracle := λ _ ↦ idOracle
 
--- @[simp]
--- lemma exec_baseOracleAlg (oa : OracleComp unifSpec α) :
---     baseOracleAlg.exec oa = oa := by
---   simp only [exec.def, idOracle.simulate'_eq]
+@[simp]
+lemma exec_baseOracleAlg (n : ℕ) (oa : OracleComp unifSpec α) :
+    baseOracleAlg.exec n oa = oa := by
+  simp only [exec_def, idOracle.simulate'_eq]
 
 end baseOracleAlg
 
